![[Pasted image 20230409122326.png]]
(a) T => D ^ Y
(b) D => $\neg$Y 
(c) $\neg$D => $\neg$T
(d) T => $\neg$(D ^ Y)
(e) T => Y ^ $\neg$D
(f) T => (Y => $\neg$D)
(g) T => (Y ^ D) v ($\neg$Y ^ $\neg$D)
(h) T => (Y v D) ^ $\neg$(Y ^ D)
![[Pasted image 20230409123642.png]]
| $\neg$$\phi$ |
 F
 F
 T
 T
| $\phi$ => $\psi$ |
	T
	F
	T
	T
| $\neg$$\phi$ V $\psi$ |
	T
	F
	T
	T
![[Pasted image 20230409124734.png]]
That the implication of an antedecent over a consequent is equivalent to the disjunction of (the negation of the antecedent) and the consequent. This means, that either the antecedent is negative or the consequent is positive in order to satisfy both conditions.
![[Pasted image 20230409124905.png]]
| $\neg$$\psi$ |
 F
 T
 F
 T
 | $\phi$ => $\psi$ |
	T
	F
	T
	T
| $\phi$ $\not$=> $\psi$ |
	F
	T
	F
	F
| $\phi$ ^ $\neg$$\psi$ |
	F
	T
	F
	F
![[Pasted image 20230409125431.png]]
That the 'not implication' of the antecedent over the consequent equals the conjunction of the antecedent with the negation of the consequent. This means, when the antecedent is True, the consequent must be false in order to satifsy both conditions.
